fixing a proof in FStar.Buffer; bump an rlimit in LowStar.Monotonic.Buffer

ulib/FStar.Buffer.fst
@@ -14,7 +14,7 @@
    limitations under the License.
 *)
 module FStar.Buffer
- 
+
 open FStar.Seq
 open FStar.UInt32
 module Int32 = FStar.Int32
@@ -28,10 +28,10 @@ module HST = FStar.HyperStack.ST
 
 #set-options "--initial_fuel 0 --max_fuel 0"
 
-//17-01-04 usage? move to UInt? 
+//17-01-04 usage? move to UInt?
 let lemma_size (x:int) : Lemma (requires (UInt.size x n))
-				     (ensures (x >= 0))
-				     [SMTPat (UInt.size x n)]
+                                     (ensures (x >= 0))
+                                     [SMTPat (UInt.size x n)]
   = ()
 
 let lseq (a: Type) (l: nat) : Type =
@@ -60,7 +60,7 @@ let max_length #a (b:buffer a) : GTot nat = v b.max_length
 let length #a (b:buffer a) : GTot nat = v b.length
 let idx #a (b:buffer a) : GTot nat = v b.idx
 
-//17-01-04 rename to container or ref? 
+//17-01-04 rename to container or ref?
 let content #a (b:buffer a) :
   GTot (reference (lseq a (max_length b))) = b.content
 
@@ -78,7 +78,7 @@ val recall: #a:Type
   (requires (fun m -> True))
   (ensures  (fun m0 _ m1 -> m0 == m1 /\ live m1 b))
 let recall #a b = recall b.content
- 
+
 (* Ghostly access an element of the array, or the full underlying sequence *)
 let as_seq #a h (b:buffer a) : GTot (s:seq a{Seq.length s == length b}) =
   Seq.slice (sel h b) (idx b) (idx b + length b)
@@ -202,7 +202,7 @@ let disjoint_3 a b b' b'' = disjoint a b /\ disjoint a b' /\ disjoint a b''
 let disjoint_4 a b b' b'' b''' = disjoint a b /\ disjoint a b' /\ disjoint a b'' /\ disjoint a b'''
 let disjoint_5 a b b' b'' b''' b'''' = disjoint a b /\ disjoint a b' /\ disjoint a b'' /\ disjoint a b''' /\ disjoint a b''''
 
-let disjoint_ref_1 (#t:Type) (#u:Type) (a:buffer t) (r:reference u) = 
+let disjoint_ref_1 (#t:Type) (#u:Type) (a:buffer t) (r:reference u) =
   frameOf a =!= HS.frameOf r \/ as_addr a =!= HS.as_addr r
 let disjoint_ref_2 a r r' = disjoint_ref_1 a r /\ disjoint_ref_1 a r'
 let disjoint_ref_3 a r r' r'' = disjoint_ref_1 a r /\ disjoint_ref_2 a r' r''
@@ -226,7 +226,7 @@ let modifies_buffers (bufs:TSet.set abuffer) h h' : GTot Type0 =
   (forall rid. Set.mem rid (Map.domain (HS.get_hmap h)) ==>
     (HS.modifies_ref rid (arefs bufs) h h' /\
       (forall (#a:Type) (b:buffer a). {:pattern (frameOf b == rid /\ live h b /\ disjoint_from_bufs b bufs)}
-	(frameOf b == rid /\ live h b /\ disjoint_from_bufs b bufs ==> equal h b h' b /\ live h' b))))
+        (frameOf b == rid /\ live h b /\ disjoint_from_bufs b bufs ==> equal h b h' b /\ live h' b))))
 
 (* General modifies clause for buffers only *)
 let modifies_bufs rid buffs h h' =
@@ -271,8 +271,8 @@ let modifies_buf_4 (#t:Type) (#t':Type) (#t'':Type) (#t''':Type) rid (b:buffer t
 (* General lemmas for the modifies_bufs clause *)
 let lemma_modifies_bufs_trans rid bufs h0 h1 h2 :
   Lemma (requires (modifies_bufs rid bufs h0 h1 /\ modifies_bufs rid bufs h1 h2))
-	(ensures (modifies_bufs rid bufs h0 h2))
-	[SMTPat (modifies_bufs rid bufs h0 h1); SMTPat (modifies_bufs rid bufs h1 h2)]
+        (ensures (modifies_bufs rid bufs h0 h2))
+        [SMTPat (modifies_bufs rid bufs h0 h1); SMTPat (modifies_bufs rid bufs h1 h2)]
  = ()
 
 let lemma_modifies_bufs_sub rid bufs subbufs h0 h1 :
@@ -297,80 +297,80 @@ let lemma_modifies_bufs_superset #a #a' h0 h1 bufs b b' = ()
 (* Specialized lemmas *)
 let modifies_trans_0_0 (rid:rid) (h0 h1 h2:mem) :
   Lemma (requires (modifies_buf_0 rid h0 h1 /\ modifies_buf_0 rid h1 h2))
-	(ensures (modifies_buf_0 rid h0 h2))
-	[SMTPat (modifies_buf_0 rid h0 h1); SMTPat (modifies_buf_0 rid h1 h2)]
+        (ensures (modifies_buf_0 rid h0 h2))
+        [SMTPat (modifies_buf_0 rid h0 h1); SMTPat (modifies_buf_0 rid h1 h2)]
  = ()
 
 let modifies_trans_1_0 (#t:Type) (rid:rid) (b:buffer t) (h0 h1 h2:mem) :
   Lemma (requires (modifies_buf_1 rid b h0 h1 /\ modifies_buf_0 rid h1 h2))
-	(ensures (modifies_buf_1 rid b h0 h2))
-	[SMTPat (modifies_buf_1 rid b h0 h1); SMTPat (modifies_buf_0 rid h1 h2)]
+        (ensures (modifies_buf_1 rid b h0 h2))
+        [SMTPat (modifies_buf_1 rid b h0 h1); SMTPat (modifies_buf_0 rid h1 h2)]
  = ()
 
 let modifies_trans_0_1 (#t:Type) (rid:rid) (b:buffer t) (h0 h1 h2:mem) :
   Lemma (requires (modifies_buf_0 rid h0 h1 /\ modifies_buf_1 rid b h1 h2))
-	(ensures (modifies_buf_1 rid b h0 h2))
-	[SMTPat (modifies_buf_0 rid h0 h1); SMTPat (modifies_buf_1 rid b h1 h2)]
+        (ensures (modifies_buf_1 rid b h0 h2))
+        [SMTPat (modifies_buf_0 rid h0 h1); SMTPat (modifies_buf_1 rid b h1 h2)]
  = ()
 
 let modifies_trans_1_1 (#t:Type) (rid:rid) (b:buffer t) (h0 h1 h2:mem) :
   Lemma (requires (modifies_buf_1 rid b h0 h1 /\ modifies_buf_1 rid b h1 h2))
-	(ensures (modifies_buf_1 rid b h0 h2))
-	[SMTPat (modifies_buf_1 rid b h0 h1); SMTPat (modifies_buf_1 rid b h1 h2)]
+        (ensures (modifies_buf_1 rid b h0 h2))
+        [SMTPat (modifies_buf_1 rid b h0 h1); SMTPat (modifies_buf_1 rid b h1 h2)]
  = ()
 
 let modifies_trans_1_1' (#t:Type) (#t':Type) (rid:rid) (b:buffer t) (b':buffer t') (h0 h1 h2:mem) :
   Lemma (requires (modifies_buf_1 rid b h0 h1 /\ modifies_buf_1 rid b' h1 h2))
-	(ensures (modifies_buf_2 rid b b' h0 h2))
-	[SMTPat (modifies_buf_1 rid b h0 h1); SMTPat (modifies_buf_1 rid b' h1 h2)]
+        (ensures (modifies_buf_2 rid b b' h0 h2))
+        [SMTPat (modifies_buf_1 rid b h0 h1); SMTPat (modifies_buf_1 rid b' h1 h2)]
  = ()
 
 let modifies_trans_2_0 (#t:Type) (#t':Type) (rid:rid) (b:buffer t) (b':buffer t') (h0 h1 h2:mem) :
   Lemma (requires (modifies_buf_2 rid b b' h0 h1 /\ modifies_buf_0 rid h1 h2))
-	(ensures (modifies_buf_2 rid b b' h0 h2))
-	[SMTPat (modifies_buf_2 rid b b' h0 h1); SMTPat (modifies_buf_0 rid h1 h2)]
+        (ensures (modifies_buf_2 rid b b' h0 h2))
+        [SMTPat (modifies_buf_2 rid b b' h0 h1); SMTPat (modifies_buf_0 rid h1 h2)]
  = ()
 
 let modifies_trans_2_1 (#t:Type) (#t':Type) (rid:rid) (b:buffer t) (b':buffer t') (h0 h1 h2:mem) :
   Lemma (requires (modifies_buf_2 rid b b' h0 h1 /\ modifies_buf_1 rid b h1 h2))
-	(ensures (modifies_buf_2 rid b b' h0 h2))
-	[SMTPat (modifies_buf_2 rid b b' h0 h1); SMTPat (modifies_buf_1 rid b h1 h2)]
+        (ensures (modifies_buf_2 rid b b' h0 h2))
+        [SMTPat (modifies_buf_2 rid b b' h0 h1); SMTPat (modifies_buf_1 rid b h1 h2)]
  = ()
 
 let modifies_trans_2_1' (#t:Type) (#t':Type) (rid:rid) (b:buffer t) (b':buffer t') (h0 h1 h2:mem) :
   Lemma (requires (modifies_buf_2 rid b' b h0 h1 /\ modifies_buf_1 rid b h1 h2))
-	(ensures (modifies_buf_2 rid b b' h0 h2))
-	[SMTPat (modifies_buf_2 rid b' b h0 h1); SMTPat (modifies_buf_1 rid b h1 h2)]
+        (ensures (modifies_buf_2 rid b b' h0 h2))
+        [SMTPat (modifies_buf_2 rid b' b h0 h1); SMTPat (modifies_buf_1 rid b h1 h2)]
  = ()
 
 let modifies_trans_0_2 (#t:Type) (#t':Type) (rid:rid) (b:buffer t) (b':buffer t') (h0 h1 h2:mem) :
   Lemma (requires (modifies_buf_0 rid h0 h1 /\ modifies_buf_2 rid b b' h1 h2))
-	(ensures (modifies_buf_2 rid b b' h0 h2))
-	[SMTPat (modifies_buf_0 rid h0 h1); SMTPat (modifies_buf_2 rid b b' h1 h2)]
+        (ensures (modifies_buf_2 rid b b' h0 h2))
+        [SMTPat (modifies_buf_0 rid h0 h1); SMTPat (modifies_buf_2 rid b b' h1 h2)]
  = ()
 
 let modifies_trans_1_2 (#t:Type) (#t':Type) (rid:rid) (b:buffer t) (b':buffer t') (h0 h1 h2:mem) :
   Lemma (requires (modifies_buf_1 rid b h0 h1 /\ modifies_buf_2 rid b b' h1 h2))
-	(ensures (modifies_buf_2 rid b b' h0 h2))
-	[SMTPat (modifies_buf_1 rid b h0 h1); SMTPat (modifies_buf_2 rid b b' h1 h2)]
+        (ensures (modifies_buf_2 rid b b' h0 h2))
+        [SMTPat (modifies_buf_1 rid b h0 h1); SMTPat (modifies_buf_2 rid b b' h1 h2)]
  = ()
 
 let modifies_trans_2_2 (#t:Type) (#t':Type) (rid:rid) (b:buffer t) (b':buffer t') (h0 h1 h2:mem) :
   Lemma (requires (modifies_buf_2 rid b b' h0 h1 /\ modifies_buf_2 rid b b' h1 h2))
-	(ensures (modifies_buf_2 rid b b' h0 h2))
-	[SMTPat (modifies_buf_2 rid b b' h0 h1); SMTPat (modifies_buf_2 rid b b' h1 h2)]
+        (ensures (modifies_buf_2 rid b b' h0 h2))
+        [SMTPat (modifies_buf_2 rid b b' h0 h1); SMTPat (modifies_buf_2 rid b b' h1 h2)]
  = ()
 
 let modifies_trans_3_3 (#t #t' #t'':Type) (rid:rid) (b:buffer t) (b':buffer t') (b'':buffer t'') (h0 h1 h2:mem) :
   Lemma (requires (modifies_buf_3 rid b b' b'' h0 h1 /\ modifies_buf_3 rid b b' b'' h1 h2))
-	(ensures (modifies_buf_3 rid b b' b'' h0 h2))
-	[SMTPat (modifies_buf_3 rid b b' b'' h0 h1); SMTPat (modifies_buf_3 rid b b' b'' h1 h2)]
+        (ensures (modifies_buf_3 rid b b' b'' h0 h2))
+        [SMTPat (modifies_buf_3 rid b b' b'' h0 h1); SMTPat (modifies_buf_3 rid b b' b'' h1 h2)]
  = ()
 
 let modifies_trans_4_4 (#t #t' #t'' #t''':Type) (rid:rid) (b:buffer t) (b':buffer t') (b'':buffer t'') (b''':buffer t''') (h0 h1 h2:mem) :
   Lemma (requires (modifies_buf_4 rid b b' b'' b''' h0 h1 /\ modifies_buf_4 rid b b' b'' b''' h1 h2))
-	(ensures (modifies_buf_4 rid b b' b'' b''' h0 h2))
-	[SMTPat (modifies_buf_4 rid b b' b'' b''' h0 h1); SMTPat (modifies_buf_4 rid b b' b'' b''' h1 h2)]
+        (ensures (modifies_buf_4 rid b b' b'' b''' h0 h2))
+        [SMTPat (modifies_buf_4 rid b b' b'' b''' h0 h1); SMTPat (modifies_buf_4 rid b b' b'' b''' h1 h2)]
  = ()
 
 (* TODO: complete with specialized versions of every general lemma *)
@@ -549,14 +549,14 @@ let lemma_reveal_modifies_3 (#a:Type) (#a':Type) (#a'':Type) (b:buffer a) (b':bu
     (let rid = frameOf b in let rid' = frameOf b' in let rid'' = frameOf b'' in
     ((rid == rid' /\ rid' == rid'' /\ modifies_buf_3 rid b b' b'' h0 h1 /\ modifies_one rid h0 h1)
     \/ (rid == rid' /\ rid' =!= rid'' /\ modifies_buf_2 rid b b' h0 h1 /\ modifies_buf_1 rid'' b'' h0 h1
-	/\ HS.modifies (Set.union (Set.singleton rid) (Set.singleton rid'')) h0 h1 )
-	\/ (rid =!= rid' /\ rid' == rid'' /\ modifies_buf_2 rid' b' b'' h0 h1 /\ modifies_buf_1 rid b h0 h1
-	/\ HS.modifies (Set.union (Set.singleton rid) (Set.singleton rid'')) h0 h1 )
-	\/ (rid == rid'' /\ rid' =!= rid'' /\ modifies_buf_2 rid b b'' h0 h1 /\ modifies_buf_1 rid' b' h0 h1
-	/\ HS.modifies (Set.union (Set.singleton rid) (Set.singleton rid')) h0 h1 )
-	\/ (rid =!= rid' /\ rid' =!= rid'' /\ rid =!= rid''
-	/\ HS.modifies (Set.union (Set.union (Set.singleton rid) (Set.singleton rid')) (Set.singleton rid'')) h0 h1
-	/\ modifies_buf_1 rid b h0 h1 /\ modifies_buf_1 rid' b' h0 h1 /\ modifies_buf_1 rid'' b'' h0 h1)) )))
+        /\ HS.modifies (Set.union (Set.singleton rid) (Set.singleton rid'')) h0 h1 )
+        \/ (rid =!= rid' /\ rid' == rid'' /\ modifies_buf_2 rid' b' b'' h0 h1 /\ modifies_buf_1 rid b h0 h1
+        /\ HS.modifies (Set.union (Set.singleton rid) (Set.singleton rid'')) h0 h1 )
+        \/ (rid == rid'' /\ rid' =!= rid'' /\ modifies_buf_2 rid b b'' h0 h1 /\ modifies_buf_1 rid' b' h0 h1
+        /\ HS.modifies (Set.union (Set.singleton rid) (Set.singleton rid')) h0 h1 )
+        \/ (rid =!= rid' /\ rid' =!= rid'' /\ rid =!= rid''
+        /\ HS.modifies (Set.union (Set.union (Set.singleton rid) (Set.singleton rid')) (Set.singleton rid'')) h0 h1
+        /\ modifies_buf_1 rid b h0 h1 /\ modifies_buf_1 rid' b' h0 h1 /\ modifies_buf_1 rid'' b'' h0 h1)) )))
   = ()
 
 let lemma_reveal_modifies_3_2 (#a:Type) (#a':Type) (b:buffer a) (b':buffer a') h0 h1 : Lemma
@@ -568,12 +568,12 @@ let lemma_reveal_modifies_3_2 (#a:Type) (#a':Type) (b:buffer a) (b':buffer a') h
     \/ (rid == rid' /\ rid' =!= HS.get_tip h0 /\ modifies_buf_2 rid b b' h0 h1 /\ modifies_buf_0 (HS.get_tip h0) h0 h1
       /\ HS.modifies (Set.union (Set.singleton rid) (Set.singleton (HS.get_tip h0))) h0 h1 )
       \/ (rid =!= rid' /\ rid == HS.get_tip h0 /\ modifies_buf_1 rid b h0 h1 /\ modifies_buf_1 rid' b' h0 h1
-	/\ HS.modifies (Set.union (Set.singleton rid') (Set.singleton (HS.get_tip h0))) h0 h1 )
-	\/ (rid =!= rid' /\ rid' == HS.get_tip h0 /\ modifies_buf_1 rid' b' h0 h1 /\ modifies_buf_1 rid b h0 h1
-	/\ HS.modifies (Set.union (Set.singleton rid) (Set.singleton (HS.get_tip h0))) h0 h1 )
-	\/ (rid =!= rid' /\ rid' =!= HS.get_tip h0 /\ rid =!= HS.get_tip h0
-	/\ HS.modifies (Set.union (Set.union (Set.singleton rid) (Set.singleton rid')) (Set.singleton (HS.get_tip h0))) h0 h1
-	/\ modifies_buf_1 rid b h0 h1 /\ modifies_buf_1 rid' b' h0 h1 /\ modifies_buf_0 (HS.get_tip h0) h0 h1)) )))
+        /\ HS.modifies (Set.union (Set.singleton rid') (Set.singleton (HS.get_tip h0))) h0 h1 )
+        \/ (rid =!= rid' /\ rid' == HS.get_tip h0 /\ modifies_buf_1 rid' b' h0 h1 /\ modifies_buf_1 rid b h0 h1
+        /\ HS.modifies (Set.union (Set.singleton rid) (Set.singleton (HS.get_tip h0))) h0 h1 )
+        \/ (rid =!= rid' /\ rid' =!= HS.get_tip h0 /\ rid =!= HS.get_tip h0
+        /\ HS.modifies (Set.union (Set.union (Set.singleton rid) (Set.singleton rid')) (Set.singleton (HS.get_tip h0))) h0 h1
+        /\ modifies_buf_1 rid b h0 h1 /\ modifies_buf_1 rid' b' h0 h1 /\ modifies_buf_0 (HS.get_tip h0) h0 h1)) )))
   = ()
 
 let lemma_reveal_modifies_region (rid:rid) bufs h0 h1 : Lemma
@@ -844,7 +844,7 @@ val createL: #a:Type0 -> init:list a -> StackInline (buffer a)
      /\ as_seq h1 b == Seq.seq_of_list init
      /\ q #a len b))
 #set-options "--initial_fuel 1 --max_fuel 1" //the normalize_term (length init) in the pre-condition will be unfolded
-	                                     //whereas the L.length init below will not
+                                             //whereas the L.length init below will not
 let createL #a init =
   let len = UInt32.uint_to_t (FStar.List.Tot.length init) in
   let s = Seq.seq_of_list init in
@@ -876,7 +876,7 @@ unfold let rcreate_post_common (#a:Type) (r:rid) (init:a) (len:UInt32.t) (b:buff
 private let rcreate_common (#a:Type) (r:rid) (init:a) (len:UInt32.t) (mm:bool)
   :ST (buffer a) (requires (fun h0      -> is_eternal_region r))
                  (ensures  (fun h0 b h1 -> rcreate_post_common r init len b h0 h1 /\
-		                        is_mm b.content == mm))
+                                        is_mm b.content == mm))
   = let h0 = HST.get() in
     let s = Seq.create (v len) init in
     let content: reference (lseq a (v len)) =
@@ -949,8 +949,8 @@ let to_seq #a b l =
 // ocaml-only, used for conversions to Platform.bytes
 val to_seq_full: #a:Type -> b:buffer a -> ST (seq a)
   (requires (fun h -> live h b))
-  (ensures  (fun h0 r h1 -> h0 == h1 /\ live h1 b /\ 
-			 r == as_seq #a h1 b ))
+  (ensures  (fun h0 r h1 -> h0 == h1 /\ live h1 b /\
+                         r == as_seq #a h1 b ))
 let to_seq_full #a b =
   let s = !b.content in
   let i = v b.idx in
@@ -970,8 +970,8 @@ private let lemma_aux_0
   (#a:Type) (b:buffer a) (n:UInt32.t{v n < length b}) (z:a) (h0:mem) (tt:Type) (bb:buffer tt)
   :Lemma (requires (live h0 b /\ live h0 bb /\ disjoint b bb))
          (ensures  (live h0 b /\ live h0 bb /\
-	            (let h1 = HS.upd h0 b.content (Seq.upd (sel h0 b) (idx b + v n) z) in
-		     as_seq h0 bb == as_seq h1 bb)))
+                    (let h1 = HS.upd h0 b.content (Seq.upd (sel h0 b) (idx b + v n) z) in
+                     as_seq h0 bb == as_seq h1 bb)))
   = Heap.lemma_distinct_addrs_distinct_preorders ();
     Heap.lemma_distinct_addrs_distinct_mm ()
 
@@ -980,9 +980,9 @@ private let lemma_aux_1
   (#a:Type) (b:buffer a) (n:UInt32.t{v n < length b}) (z:a) (h0:mem) (tt:Type)
   :Lemma (requires (live h0 b))
          (ensures  (live h0 b /\
-	            (forall (bb:buffer tt). (live h0 bb /\ disjoint b bb) ==>
-		                       (let h1 = HS.upd h0 b.content (Seq.upd (sel h0 b) (idx b + v n) z) in
-		                        as_seq h0 bb == as_seq h1 bb))))
+                    (forall (bb:buffer tt). (live h0 bb /\ disjoint b bb) ==>
+                                       (let h1 = HS.upd h0 b.content (Seq.upd (sel h0 b) (idx b + v n) z) in
+                                        as_seq h0 bb == as_seq h1 bb))))
   = let open FStar.Classical in
     forall_intro (move_requires (lemma_aux_0 b n z h0 tt))
 
@@ -992,9 +992,9 @@ private let lemma_aux_2
   (#a:Type) (b:buffer a) (n:UInt32.t{v n < length b}) (z:a) (h0:mem)
   :Lemma (requires (live h0 b))
          (ensures  (live h0 b /\
-	            (forall (tt:Type) (bb:buffer tt). (live h0 bb /\ disjoint b bb) ==>
-		                                 (let h1 = HS.upd h0 b.content (Seq.upd (sel h0 b) (idx b + v n) z) in
-		                                  as_seq h0 bb == as_seq h1 bb))))
+                    (forall (tt:Type) (bb:buffer tt). (live h0 bb /\ disjoint b bb) ==>
+                                                 (let h1 = HS.upd h0 b.content (Seq.upd (sel h0 b) (idx b + v n) z) in
+                                                  as_seq h0 bb == as_seq h1 bb))))
   = let open FStar.Classical in
     forall_intro (move_requires (lemma_aux_1 b n z h0))
 
@@ -1037,7 +1037,7 @@ let sub_sub
   (len2: UInt32.t {v i2 + v len2 <= v len1})
 : Lemma
   (ensures (sub (sub b i1 len1) i2 len2 == sub b (i1 +^ i2) len2))
-= ()  
+= ()
 
 let sub_zero_length
   (#a: Type)
@@ -1080,7 +1080,7 @@ let lemma_offset_spec (#a:Type) (b:buffer a)
      [SMTPatOr [[SMTPat (as_seq h (offset b i))];
                 [SMTPat (Seq.slice (as_seq h b) (v i) (length b))]]]
   = Seq.lemma_eq_intro (as_seq h (offset b i)) (Seq.slice (as_seq h b) (v i) (length b))
-  
+
 private val eq_lemma1:
     #a:eqtype
   -> b1:buffer a
@@ -1195,22 +1195,29 @@ val fill: #t:Type
     (requires (fun h -> live h b))
     (ensures  (fun h0 _ h1 -> live h0 b /\ live h1 b /\ modifies_1 b h0 h1
       /\ Seq.slice (as_seq h1 b) 0 (v len) == Seq.create (v len) z
-      /\ Seq.slice (as_seq h1 b) (v len) (length b) ==
-        Seq.slice (as_seq h0 b) (v len) (length b) ))
+      /\ (Seq.slice (as_seq h1 b) (v len) (length b) ==
+         Seq.slice (as_seq h0 b) (v len) (length b) )))
+
 let rec fill #t b z len =
   let h0 = HST.get () in
-  if len =^ 0ul then ()
+  if len =^ 0ul
+  then
+    begin
+       Seq.lemma_eq_intro (Seq.slice (as_seq h0 b) 0 (v len))
+                          (Seq.create (v len) z)
+    end
   else
     begin
     let len' = len -^ 1ul in
     fill #t b z len';
+    let h1 = HST.get () in
+    Seq.lemma_tail_slice (as_seq h1 b) (v len') (length b);
     b.(len') <- z;
-    let h = HST.get() in
-    Seq.snoc_slice_index (as_seq h b) 0 (v len');
-    Seq.lemma_tail_slice (as_seq h b) (v len') (length b)
-    end;
-  let h1 = HST.get() in
-  Seq.lemma_eq_intro (Seq.slice (as_seq h1 b) 0 (v len)) (Seq.create (v len) z)
+    let h2 = HST.get() in
+    Seq.snoc_slice_index (as_seq h2 b) 0 (v len');
+    Seq.lemma_eq_intro (Seq.slice (as_seq h2 b) 0 (v len))
+                       (Seq.create (v len) z)
+    end
 
 
 let split #t (b:buffer t) (i:UInt32.t{v i <= length b}) : Tot (buffer t * buffer t)
@@ -1296,7 +1303,7 @@ let modifies_subbuffer_2 (#t:Type) (#t':Type) h0 h1 (sub:buffer t) (a':buffer t'
   (ensures  (modifies_2 a a' h0 h1 /\ modifies_2 a' a h0 h1 /\ live h1 a))
   [SMTPat (modifies_2 sub a' h0 h1); SMTPat (includes a sub)]
   = ()
-    
+
 let modifies_subbuffer_2' (#t:Type) (#t':Type) h0 h1 (sub:buffer t) (a':buffer t') (a:buffer t) : Lemma
   (requires (live h0 a /\ live h0 a' /\ includes a sub /\ modifies_2 a' sub h0 h1 ))
   (ensures  (modifies_2 a a' h0 h1 /\ live h1 a))
